

Also, we can look at the situations where  $\theta$  affects the dynamics classically. This occurs when  $\theta$  is not constant, but instead, varies in space and time.

$$\theta = \theta(\vec{x}, t).$$

So we can ~~not~~ write down the axion electrodynamics action:

$$S = \int d^4x \left( -\frac{1}{4} F^{\mu\nu} F_{\mu\nu} + \frac{e^2}{16\pi^2} \theta(\vec{x}, t) \cdot F^{\mu\nu} \cdot F_{\mu\nu} \right)$$

We use Euler-Lagrange equations: ~~to~~

$$\frac{\partial \mathcal{L}}{\partial A_\mu} - \partial_\nu \left( \frac{\partial \mathcal{L}}{\partial (\partial_\nu A_\mu)} \right) = 0$$

to get the equations of axion electrodynamics

Because  $\mathcal{L}$  doesn't depend on  $A_\mu$ , so the equations of motion are:

$$\frac{\partial \mathcal{L}}{\partial A_\mu} = 0 \Rightarrow \partial_\nu \left( \frac{\partial \mathcal{L}}{\partial (\partial_\nu A_\mu)} \right) = 0$$

and the  $\mathcal{L}$  of axion electrodynamics is ( $\alpha = \frac{e^2}{4\pi}$ ):

$$\mathcal{L} = \mathcal{L}_{\text{max}} + \mathcal{L}_\theta$$

$$= -\frac{1}{4} F^{\mu\nu} F_{\mu\nu} + \frac{\alpha}{4\pi} \theta(\vec{x}, t) \cdot F^{\mu\nu} F_{\mu\nu}$$

First, let's see  $\mathcal{L}_0$ :

$$\begin{aligned} \frac{\partial \mathcal{L}}{\partial (\partial_\nu A_\mu)} &= \frac{\partial}{\partial (\partial_\nu A_\mu)} \cdot \frac{\alpha}{4\lambda} \theta(\vec{x}, t) \cdot \cancel{\epsilon^{\mu\nu\rho\sigma} F_{\rho\sigma} F_{\mu\nu}} \\ &= \frac{\alpha}{4\lambda} \left\{ \frac{\partial}{\partial (\partial_\nu A_\mu)} \cdot \theta(\vec{x}, t) \right\} \cdot \epsilon^{\alpha\beta\rho\sigma} F_{\alpha\beta} F_{\rho\sigma} + \theta(\vec{x}, t) \left[ \frac{\partial \epsilon^{\alpha\beta\rho\sigma} F_{\alpha\beta} F_{\rho\sigma}}{\partial (\partial_\nu A_\mu)} \right] \end{aligned}$$

let's see the first term.

$$\epsilon^{\alpha\beta\rho\sigma} F_{\alpha\beta} F_{\rho\sigma} \frac{\partial}{\partial (\partial_\nu A_\mu)} \theta(\vec{x}, t) = 0$$

then let's see the second term:

$$\begin{aligned} &\theta(\vec{x}, t) \cdot \frac{\partial}{\partial (\partial_\nu A_\mu)} \cdot \epsilon^{\alpha\beta\rho\sigma} F_{\alpha\beta} F_{\rho\sigma} = \theta(\vec{x}, t) \cdot \\ &= 4\theta(\vec{x}, t) \left( \frac{\partial}{\partial (\partial_\nu A_\mu)} \cdot \partial_\alpha A_\beta \partial_\rho A_\sigma \right) \epsilon^{\alpha\beta\rho\sigma} \\ &= 4\theta(\vec{x}, t) \left( \delta_\alpha^\nu \delta_\beta^\mu \partial_\rho A_\sigma + \delta_\rho^\nu \delta_\sigma^\mu \partial_\alpha A_\beta \right) \epsilon^{\alpha\beta\rho\sigma} \\ &= 4\theta(\vec{x}, t) \cdot \epsilon^{\nu\mu\rho\sigma} (\partial_\rho A_\sigma - \partial_\sigma A_\rho) \\ &= 8\theta(\vec{x}, t) \star F^{\nu\mu} \end{aligned}$$

next, we can get:

$$\partial_\nu (\theta(\vec{x}, t) \star F^{\nu\mu}) = \star F^{\nu\mu} \partial_\nu \theta(\vec{x}, t) + \theta(\vec{x}, t) \cdot \partial_\nu \star F^{\nu\mu}$$

using the Bianchi identities:

$$\partial_\mu \star F^{\mu\nu} = 0$$

so we can get:

$$\partial_\nu \theta(\vec{x}, t) {}^\star F^{\nu\mu} = {}^\star F^{\nu\mu} \partial_\nu \theta(\vec{x}, t)$$

~~Finally, we can~~ Finally, we can get:

$$\partial_\nu \left( \frac{\partial \mathcal{L}_\theta}{\partial (\partial_\nu A_\mu)} \right) = \frac{\alpha}{\pi} {}^\star F^{\nu\mu} \cdot \partial_\nu \theta(\vec{x}, t)$$

\* And the Lagrangian of Maxwell part:

$$\partial_\nu \left( \frac{\partial \mathcal{L}_{\text{Max}}}{\partial (\partial_\nu A_\mu)} \right) = - \partial_\nu F^{\nu\mu}.$$

So the equations of axion electrodynamics is.

$$\begin{cases} \partial_\nu F^{\nu\mu} = \frac{\alpha}{\pi} {}^\star F^{\nu\mu} \cdot \partial_\nu \theta(\vec{x}, t) \\ \partial_\mu {}^\star F^{\mu\nu} = 0 \end{cases}$$

In the end, the deformed Maxwell equations <sup>which</sup> are ~~the~~ the equations of axion electrodynamics are:

$$\begin{cases} \nabla \cdot \vec{E} = \frac{\alpha}{\pi} (\nabla \cdot \vec{\theta}) \cdot \vec{B} \\ \nabla \times \vec{B} = \frac{\partial \vec{E}}{\partial t} + \frac{\alpha}{\pi} (\vec{\theta} \vec{B} + \nabla \theta \times \vec{E}) \\ \nabla \cdot \vec{B} = 0 \\ \frac{\partial \vec{B}}{\partial t} + \nabla \times \vec{E} = 0 \end{cases}$$